nicer specs and naming, straightline_call now super slow but proofs in ladderstep work eventually

src/Bedrock/Synthesis/Examples/X25519_64.v
@@ -1,6 +1,7 @@
 Require Import Coq.ZArith.ZArith.
 Require Import Coq.Lists.List.
 Require Import Coq.Strings.String.
+Require Import Crypto.Bedrock.Parameters.SelectParameters.
 Require Import Crypto.Bedrock.Interfaces.UnsaturatedSolinas.
 Require Import Crypto.Bedrock.Synthesis.UnsaturatedSolinas.
 Local Open Scope Z_scope.
@@ -12,21 +13,29 @@ Let c := [(1, 19)].
 Let machine_wordsize := 64.
 Let prefix := "curve25519_"%string. (* placed before function names *)
 
-Instance names : names_of_operations.
+Definition names : names_of_operations.
 make_names_of_operations prefix. Defined.
 
-Instance p : Types.parameters.
-make_parameters machine_wordsize. Defined.
-Instance p_ok : Types.ok. typeclasses eauto. Qed.
-
 Local Instance curve25519_bedrock2_scmul121665
-  : bedrock2_unsaturated_solinas_scmul n s c 121665.
-Proof. make_bedrock2_unsaturated_solinas_scmul. Defined.
+  : bedrock2_unsaturated_solinas_scmul 121665.
+Proof.
+  let p := parameters_from_wordsize machine_wordsize in
+  make_bedrock2_unsaturated_solinas_scmul p names n s c machine_wordsize.
+Defined.
 
 Local Instance curve25519_bedrock2_scmul121666
-  : bedrock2_unsaturated_solinas_scmul n s c 121666.
-Proof. make_bedrock2_unsaturated_solinas_scmul. Defined.
+  : bedrock2_unsaturated_solinas_scmul 121666.
+Proof.
+  let p := parameters_from_wordsize machine_wordsize in
+  make_bedrock2_unsaturated_solinas_scmul p names n s c machine_wordsize.
+Defined.
 
-Instance curve25519_bedrock2 : bedrock2_unsaturated_solinas n s c.
-Proof. make_bedrock2_unsaturated_solinas. Time Defined.
-(* Eval cbv [carry_mul curve25519_bedrock2] in carry_mul. *)
+Instance curve25519_bedrock2 : bedrock2_unsaturated_solinas.
+Proof.
+  let p := parameters_from_wordsize machine_wordsize in
+  make_bedrock2_unsaturated_solinas p names n s c machine_wordsize.
+Time Defined.
+(*
+Eval cbv [add curve25519_bedrock2] in add.
+Eval cbv [spec_of_add curve25519_bedrock2] in spec_of_add.
+*)
